proofs/fstar/extraction/Sandwich.Error.Code.fst
@@ -23,6 +23,14 @@ let impl_41: t_AllowedProtoBasedErrorCodeEnum Sandwich_proto.Errors.t_TLSConfigu
     _super_9442900250278684536 = FStar.Tactics.Typeclasses.solve
   }
 
+/// Adds `ErrorEnum` to the list of [`AllowedProtoBasedErrorCodeEnum`] trait.
+[@@ FStar.Tactics.Typeclasses.tcinstance]
+let impl_131: t_AllowedProtoBasedErrorCodeEnum Sandwich_proto.Errors.t_TunnelError =
+  {
+    _super_11581440318597584651 = FStar.Tactics.Typeclasses.solve;
+    _super_9442900250278684536 = FStar.Tactics.Typeclasses.solve
+  }
+
 /// An error code.
 /// An error code holds one of the error described in `errors.proto`
 /// and listed in `ErrorKind`.
@@ -61,6 +69,20 @@ let impl_36: Core.Convert.t_From t_ProtoBasedErrorCode Sandwich_proto.Errors.t_T
     =
     fun (v: Sandwich_proto.Errors.t_TLSConfigurationError) ->
       ProtoBasedErrorCode_TLSConfigurationError v <: t_ProtoBasedErrorCode
+  }
+
+/// Implements `[From<sandwich_proto::ErrorEnum>]` for [`ProtoBasedErrorCode`].
+[@@ FStar.Tactics.Typeclasses.tcinstance]
+let impl_126: Core.Convert.t_From t_ProtoBasedErrorCode Sandwich_proto.Errors.t_TunnelError =
+  {
+    f_from_pre = (fun (v: Sandwich_proto.Errors.t_TunnelError) -> true);
+    f_from_post
+    =
+    (fun (v: Sandwich_proto.Errors.t_TunnelError) (out: t_ProtoBasedErrorCode) -> true);
+    f_from
+    =
+    fun (v: Sandwich_proto.Errors.t_TunnelError) ->
+      ProtoBasedErrorCode_TunnelError v <: t_ProtoBasedErrorCode
   }
 
 /// An error code.
@@ -113,6 +135,35 @@ let impl_39: Core.Convert.t_From t_ErrorCode
         =
         Core.Convert.f_from #t_ProtoBasedErrorCode
           #Sandwich_proto.Errors.t_TLSConfigurationError
+          #FStar.Tactics.Typeclasses.solve
+          v;
+        f_msg
+        =
+        Core.Option.Option_Some
+        (Core.Convert.f_into #string #Alloc.String.t_String #FStar.Tactics.Typeclasses.solve s)
+        <:
+        Core.Option.t_Option Alloc.String.t_String
+      }
+      <:
+      t_ErrorCode
+  }
+
+/// Instantiates an [`ErrorCode`] from an error enum and a string.
+[@@ FStar.Tactics.Typeclasses.tcinstance]
+let impl_129: Core.Convert.t_From t_ErrorCode (Sandwich_proto.Errors.t_TunnelError & string) =
+  {
+    f_from_pre = (fun (v, s: (Sandwich_proto.Errors.t_TunnelError & string)) -> true);
+    f_from_post
+    =
+    (fun (v, s: (Sandwich_proto.Errors.t_TunnelError & string)) (out: t_ErrorCode) -> true);
+    f_from
+    =
+    fun (v, s: (Sandwich_proto.Errors.t_TunnelError & string)) ->
+      {
+        f_ec
+        =
+        Core.Convert.f_from #t_ProtoBasedErrorCode
+          #Sandwich_proto.Errors.t_TunnelError
           #FStar.Tactics.Typeclasses.solve
           v;
         f_msg
